

# Homework1

Saturday, August 24, 2024

6:40 PM

1)

$$A = \begin{bmatrix} 4 & 1 & 8 \\ 2 & -7 & 5 \end{bmatrix}_{2 \times 3} \quad B = \begin{bmatrix} -9 & 7 \\ 1 & 5 \\ 8 & 3 \end{bmatrix}_{3 \times 2}$$

a)  $AB$

$$\begin{bmatrix} (4 \times -9) + (1 \times 1) + (8 \times 8) & (4 \times 7) + (1 \times 5) + (8 \times 3) \\ (2 \times -9) + (-7 \times 1) + (5 \times 8) & (2 \times 7) + (-7 \times 5) + (5 \times 3) \end{bmatrix} = \begin{bmatrix} 29 & 57 \\ 15 & -6 \end{bmatrix}$$

b)

$$BA = \begin{bmatrix} -9 & 7 \\ 1 & 5 \\ 8 & 3 \end{bmatrix} \times \begin{bmatrix} 4 & 1 & 8 \\ 2 & -7 & 5 \end{bmatrix} = \begin{bmatrix} -22 & -58 & -37 \\ 14 & -34 & 33 \\ 38 & -13 & 79 \end{bmatrix}$$

c)

$$-B = -1 \cdot B = \begin{bmatrix} 9 & -7 \\ -1 & -5 \\ -8 & -3 \end{bmatrix}$$

d)

To sum or subtract matrices, both have to have the same dimensions, in this case  $A(2 \times 3)$  and  $B(3 \times 2)$  don't

e)

$$A^T = \begin{bmatrix} 4 & 2 \\ 1 & -7 \\ 8 & 5 \end{bmatrix}$$

f)  $-B^T \cdot B$

$$\begin{bmatrix} 9 & -1 & -8 \\ -7 & -5 & -3 \end{bmatrix} \begin{bmatrix} -9 & 7 \\ 1 & 5 \\ 8 & 3 \end{bmatrix}$$

$$\begin{bmatrix} (9 \times -9) + (-1 \times 1) + (-8 \times 8) & (9 \times 7) + (-1 \times 5) + (-8 \times 3) \\ (-7 \times -9) + (-5 \times 1) + (-3 \times 8) & (-7 \times 7) + (-5 \times 5) + (-3 \times 3) \end{bmatrix}$$

$$= \begin{bmatrix} 148 & -34 \\ -34 & 83 \end{bmatrix}$$

2)

a)

$$15x + 5y = 25 \quad (1) \rightarrow (1) - (2) = 7x = 23$$

$$3x + 5y = 2 \quad (2)$$

$$x = \frac{23}{7}$$

$$8\left(\frac{23}{7}\right) + 5y = 2 \rightarrow y = \frac{-34}{7}$$

b)

$$3x + y = 8 \quad (1) \quad (1) + (2) = 6x = 16 \rightarrow x = \frac{16}{6}$$

$$3x - y = 8 \quad (2)$$

$$3\left(\frac{16}{6}\right) - y = 8 \rightarrow y = 0$$

c)

$$2x - 24y = 42 \quad (1)$$

$$-2x + 24y = -40 \quad (2)$$

$$(1) + (2) = 0 = 2 \rightarrow \text{contradiction}$$

the contradiction is because the equations are parallel lines that never intersect

3)

a)

$$C = \begin{bmatrix} 7 & -2 \\ 12 & -8 \end{bmatrix}$$

$$C^{-1} = \frac{1}{\det C} \cdot \begin{bmatrix} d & -b \\ -c & a \end{bmatrix}$$

$C^{-1} = \frac{1}{0} \rightarrow$  since the determinant is zero, the matrix  $C$  doesn't have an inverse

b)

$$D = \begin{bmatrix} -1 & 4 \\ 6 & -8 \end{bmatrix} \quad D^{-1} = \frac{1}{-16} \begin{bmatrix} -8 & -4 \\ -6 & -1 \end{bmatrix} = \begin{bmatrix} 8/16 & 4/16 \\ 6/16 & 1/16 \end{bmatrix}$$

c)

$$E = \begin{bmatrix} 1 & 2 & 3 \\ 4 & 5 & 6 \\ 7 & 8 & 9 \end{bmatrix} \quad \det E = 1(5 \times 9 - 6 \times 8) - 2(4 \times 9 - 6 \times 7) + 3(4 \times 8 - 5 \times 7)$$

$\det E = 0$  hence matrix  $E$  does not have an inverse

d)

$$F = \begin{bmatrix} -3 & 5 & 9 \\ 8 & -2 & 5 \\ 1 & -2 & 14 \end{bmatrix} \quad \det F = -3(-2 \times 14 + 5 \times 2) - 5(8 \times 14 - 5 \times 1) + 9(8 \times -2 + 2 \times 1) = -607$$

$$F^{-1} = \frac{1}{-607} \cdot \text{adj}(F)$$

$$\begin{vmatrix} -2 & 5 \\ -2 & 14 \end{vmatrix} = -18$$

$$\begin{vmatrix} 8 & 5 \\ 1 & 14 \end{vmatrix} = 107$$

$$\begin{vmatrix} 8 & -2 \\ 1 & -2 \end{vmatrix} = -14$$

$$\begin{vmatrix} 5 & 9 \\ -2 & 14 \end{vmatrix} = 88$$

$$\begin{vmatrix} -3 & 9 \\ 1 & 14 \end{vmatrix} = -51$$

$$\begin{vmatrix} -3 & 5 \\ 1 & -2 \end{vmatrix} = 1$$

$$\begin{vmatrix} 5 & 9 \\ -2 & 5 \end{vmatrix} = 43$$

$$\begin{vmatrix} -3 & 9 \\ 8 & 5 \end{vmatrix} = -87$$

$$\begin{vmatrix} -3 & 5 \\ 8 & -2 \end{vmatrix} = -34$$

$$\text{adj}(F) = \begin{bmatrix} -18 & -107 & -14 \\ -88 & -51 & -1 \\ 43 & 87 & -34 \end{bmatrix}$$

$$F^{-1} = \begin{bmatrix} \frac{-18}{-607} & \frac{-107}{-607} & \frac{-14}{-607} \\ \frac{-88}{-607} & \frac{-51}{-607} & \frac{-1}{-607} \\ \frac{-43}{-607} & \frac{-87}{-607} & \frac{-34}{-607} \end{bmatrix}$$

4)

a)  $\sum_{j \in \mathbb{R}} j$  : "Summation of all  $j$  where  $j$  belongs to the real numbers"

b)  $\sum_{j \in \mathbb{Z}^+, \text{mod } 5 = 0} j$  : "Sum of all  $j$  where  $j$  are all positive integers that are divisible by 5"

c)  $\sum_{\substack{j=1 \\ j \in \mathbb{Z}}}^{40} j$  : "Sum of elements  $j$  from  $j$  equal 1 to  $j$  equal 40 where  $j$  are integers"

5)

$$a) \sum_{j \in \mathbb{Z}, \text{mod } 2 \neq 0} j$$

$$b) \sum_{i \in I} \sum_{j \in J} x_{ij}$$

$$c) \sum_{i \in J} \sum_{j \in I} x_{ij} \quad (i, j) \in A$$

6)

a)  $\sum_{j \in \{0, 1, 2, \dots, 12\} : j \text{ mod } 2 = 0} j$  : this means that from the set we will only select the even numbers

$$\text{so the sum would be } = 0 + 2 + 4 + 6 + 8 + 10 + 12 = 42$$

b)

$$N = \{1, 2, 3, 4\}, A = \{(1, 2), (2, 3), (2, 4), (3, 4), (2, 1)\}, D = \{3\}, S = \{1, 2\}, T = \{4\}$$

$$b_i = \begin{cases} \alpha_i & i \in S \\ \beta_i & i \in D \quad \forall i \in N \\ 0 & i \in T \end{cases}$$

Expand:

$$\sum_{j \in N: (i, j) \in A} x_{ij} - \sum_{j \in N: (j, i) \in A} x_{ji} = b_i \quad \forall i \in N$$

for  $i = 1 (i \in S)$ :

outgoing edges :  $(1, 2)$

incoming edges :  $(2, 1)$

$$x_{12} - x_{21} = \alpha_1$$

for  $i = 2 (i \in S)$

outgoing edges :  $(2, 3), (2, 4), (2, 1)$

incoming edges :  $(1, 2)$

$$x_{21} + x_{23} + x_{24} - x_{12} = \alpha_2$$

for  $i = 3 (i \in D)$

outgoing edges :  $(3, 4)$

incoming edges :  $(2, 3)$

$$x_{34} - x_{23} = \beta_3$$

for  $i = 4 (i \in T)$

outgoing : None (No  $(4, j)$  pairs in  $A$ )

incoming :  $(2, 4), (3, 4)$

$$-x_{24} - x_{34} = 0$$

Set of equations :

$$x_{12} - x_{21} = \alpha_1$$

$$-x_{12} + x_{21} + x_{23} + x_{24} = \alpha_2$$

$$x_{34} - x_{23} = \beta_3$$

$$-x_{24} - x_{34} = 0$$